.lake/build/ir/DeepArithmetic/Semantics/ManySorted.c
@@ -1,0 +1,160 @@
+// Lean compiler output
+// Module: DeepArithmetic.Semantics.ManySorted
+// Imports: public import Init public meta import Init
+#include <lean/lean.h>
+#if defined(__clang__)
+#pragma clang diagnostic ignored "-Wunused-parameter"
+#pragma clang diagnostic ignored "-Wunused-label"
+#elif defined(__GNUC__) && !defined(__CLANG__)
+#pragma GCC diagnostic ignored "-Wunused-parameter"
+#pragma GCC diagnostic ignored "-Wunused-label"
+#pragma GCC diagnostic ignored "-Wunused-but-set-variable"
+#endif
+#ifdef __cplusplus
+extern "C" {
+#endif
+LEAN_EXPORT lean_object* lp_DeepArithmetic_DeepArithmetic_Semantics_ManySorted_extract1___redArg(lean_object*);
+LEAN_EXPORT lean_object* lp_DeepArithmetic_DeepArithmetic_Semantics_ManySorted_extract1(lean_object*, lean_object*, lean_object*);
+LEAN_EXPORT lean_object* lp_DeepArithmetic_DeepArithmetic_Semantics_ManySorted_extract2___redArg(lean_object*);
+LEAN_EXPORT lean_object* lp_DeepArithmetic_DeepArithmetic_Semantics_ManySorted_extract2(lean_object*, lean_object*, lean_object*);
+LEAN_EXPORT lean_object* lp_DeepArithmetic_DeepArithmetic_Semantics_ManySorted_extract1___redArg(lean_object* v_x_1_){
+_start:
+{
+if (lean_obj_tag(v_x_1_) == 0)
+{
+lean_object* v_val_2_; lean_object* v___x_4_; uint8_t v_isShared_5_; uint8_t v_isSharedCheck_9_; 
+v_val_2_ = lean_ctor_get(v_x_1_, 0);
+v_isSharedCheck_9_ = !lean_is_exclusive(v_x_1_);
+if (v_isSharedCheck_9_ == 0)
+{
+v___x_4_ = v_x_1_;
+v_isShared_5_ = v_isSharedCheck_9_;
+goto v_resetjp_3_;
+}
+else
+{
+lean_inc(v_val_2_);
+lean_dec(v_x_1_);
+v___x_4_ = lean_box(0);
+v_isShared_5_ = v_isSharedCheck_9_;
+goto v_resetjp_3_;
+}
+v_resetjp_3_:
+{
+lean_object* v___x_7_; 
+if (v_isShared_5_ == 0)
+{
+lean_ctor_set_tag(v___x_4_, 1);
+v___x_7_ = v___x_4_;
+goto v_reusejp_6_;
+}
+else
+{
+lean_object* v_reuseFailAlloc_8_; 
+v_reuseFailAlloc_8_ = lean_alloc_ctor(1, 1, 0);
+lean_ctor_set(v_reuseFailAlloc_8_, 0, v_val_2_);
+v___x_7_ = v_reuseFailAlloc_8_;
+goto v_reusejp_6_;
+}
+v_reusejp_6_:
+{
+return v___x_7_;
+}
+}
+}
+else
+{
+lean_object* v___x_10_; 
+lean_dec_ref_known(v_x_1_, 1);
+v___x_10_ = lean_box(0);
+return v___x_10_;
+}
+}
+}
+LEAN_EXPORT lean_object* lp_DeepArithmetic_DeepArithmetic_Semantics_ManySorted_extract1(lean_object* v_A_11_, lean_object* v_B_12_, lean_object* v_x_13_){
+_start:
+{
+lean_object* v___x_14_; 
+v___x_14_ = lp_DeepArithmetic_DeepArithmetic_Semantics_ManySorted_extract1___redArg(v_x_13_);
+return v___x_14_;
+}
+}
+LEAN_EXPORT lean_object* lp_DeepArithmetic_DeepArithmetic_Semantics_ManySorted_extract2___redArg(lean_object* v_x_15_){
+_start:
+{
+if (lean_obj_tag(v_x_15_) == 0)
+{
+lean_object* v___x_16_; 
+lean_dec_ref_known(v_x_15_, 1);
+v___x_16_ = lean_box(0);
+return v___x_16_;
+}
+else
+{
+lean_object* v_val_17_; lean_object* v___x_19_; uint8_t v_isShared_20_; uint8_t v_isSharedCheck_24_; 
+v_val_17_ = lean_ctor_get(v_x_15_, 0);
+v_isSharedCheck_24_ = !lean_is_exclusive(v_x_15_);
+if (v_isSharedCheck_24_ == 0)
+{
+v___x_19_ = v_x_15_;
+v_isShared_20_ = v_isSharedCheck_24_;
+goto v_resetjp_18_;
+}
+else
+{
+lean_inc(v_val_17_);
+lean_dec(v_x_15_);
+v___x_19_ = lean_box(0);
+v_isShared_20_ = v_isSharedCheck_24_;
+goto v_resetjp_18_;
+}
+v_resetjp_18_:
+{
+lean_object* v___x_22_; 
+if (v_isShared_20_ == 0)
+{
+v___x_22_ = v___x_19_;
+goto v_reusejp_21_;
+}
+else
+{
+lean_object* v_reuseFailAlloc_23_; 
+v_reuseFailAlloc_23_ = lean_alloc_ctor(1, 1, 0);
+lean_ctor_set(v_reuseFailAlloc_23_, 0, v_val_17_);
+v___x_22_ = v_reuseFailAlloc_23_;
+goto v_reusejp_21_;
+}
+v_reusejp_21_:
+{
+return v___x_22_;
+}
+}
+}
+}
+}
+LEAN_EXPORT lean_object* lp_DeepArithmetic_DeepArithmetic_Semantics_ManySorted_extract2(lean_object* v_A_25_, lean_object* v_B_26_, lean_object* v_x_27_){
+_start:
+{
+lean_object* v___x_28_; 
+v___x_28_ = lp_DeepArithmetic_DeepArithmetic_Semantics_ManySorted_extract2___redArg(v_x_27_);
+return v___x_28_;
+}
+}
+lean_object* initialize_Init(uint8_t builtin);
+lean_object* initialize_Init(uint8_t builtin);
+static bool _G_initialized = false;
+LEAN_EXPORT lean_object* initialize_DeepArithmetic_DeepArithmetic_Semantics_ManySorted(uint8_t builtin) {
+lean_object * res;
+if (_G_initialized) return lean_io_result_mk_ok(lean_box(0));
+_G_initialized = true;
+res = initialize_Init(builtin);
+if (lean_io_result_is_error(res)) return res;
+lean_dec_ref(res);
+res = initialize_Init(builtin);
+if (lean_io_result_is_error(res)) return res;
+lean_dec_ref(res);
+return lean_io_result_mk_ok(lean_box(0));
+}
+#ifdef __cplusplus
+}
+#endif
