.lake/build/ir/DeepArithmetic/Semantics/Peano/System.c
@@ -1,0 +1,70 @@
+// Lean compiler output
+// Module: DeepArithmetic.Semantics.Peano.System
+// Imports: public import Init public meta import Init public import DeepArithmetic.Semantics.FreeInductiveAlgebra
+#include <lean/lean.h>
+#if defined(__clang__)
+#pragma clang diagnostic ignored "-Wunused-parameter"
+#pragma clang diagnostic ignored "-Wunused-label"
+#elif defined(__GNUC__) && !defined(__CLANG__)
+#pragma GCC diagnostic ignored "-Wunused-parameter"
+#pragma GCC diagnostic ignored "-Wunused-label"
+#pragma GCC diagnostic ignored "-Wunused-but-set-variable"
+#endif
+#ifdef __cplusplus
+extern "C" {
+#endif
+LEAN_EXPORT lean_object* lp_DeepArithmetic_DeepArithmetic_Semantics_Peano_PeanoSystem_zero(lean_object*);
+LEAN_EXPORT lean_object* lp_DeepArithmetic_DeepArithmetic_Semantics_Peano_PeanoSystem_zero___boxed(lean_object*);
+LEAN_EXPORT lean_object* lp_DeepArithmetic_DeepArithmetic_Semantics_Peano_PeanoSystem_succ(lean_object*, lean_object*);
+LEAN_EXPORT lean_object* lp_DeepArithmetic_DeepArithmetic_Semantics_Peano_PeanoSystem_zero(lean_object* v_S_1_){
+_start:
+{
+lean_object* v_base_2_; 
+v_base_2_ = lean_ctor_get(v_S_1_, 0);
+lean_inc(v_base_2_);
+return v_base_2_;
+}
+}
+LEAN_EXPORT lean_object* lp_DeepArithmetic_DeepArithmetic_Semantics_Peano_PeanoSystem_zero___boxed(lean_object* v_S_3_){
+_start:
+{
+lean_object* v_res_4_; 
+v_res_4_ = lp_DeepArithmetic_DeepArithmetic_Semantics_Peano_PeanoSystem_zero(v_S_3_);
+lean_dec_ref(v_S_3_);
+return v_res_4_;
+}
+}
+LEAN_EXPORT lean_object* lp_DeepArithmetic_DeepArithmetic_Semantics_Peano_PeanoSystem_succ(lean_object* v_S_5_, lean_object* v_n_6_){
+_start:
+{
+lean_object* v_step_7_; lean_object* v___x_8_; lean_object* v___x_9_; 
+v_step_7_ = lean_ctor_get(v_S_5_, 1);
+lean_inc(v_step_7_);
+lean_dec_ref(v_S_5_);
+v___x_8_ = lean_box(0);
+v___x_9_ = lean_apply_2(v_step_7_, v___x_8_, v_n_6_);
+return v___x_9_;
+}
+}
+lean_object* initialize_Init(uint8_t builtin);
+lean_object* initialize_Init(uint8_t builtin);
+lean_object* initialize_DeepArithmetic_DeepArithmetic_Semantics_FreeInductiveAlgebra(uint8_t builtin);
+static bool _G_initialized = false;
+LEAN_EXPORT lean_object* initialize_DeepArithmetic_DeepArithmetic_Semantics_Peano_System(uint8_t builtin) {
+lean_object * res;
+if (_G_initialized) return lean_io_result_mk_ok(lean_box(0));
+_G_initialized = true;
+res = initialize_Init(builtin);
+if (lean_io_result_is_error(res)) return res;
+lean_dec_ref(res);
+res = initialize_Init(builtin);
+if (lean_io_result_is_error(res)) return res;
+lean_dec_ref(res);
+res = initialize_DeepArithmetic_DeepArithmetic_Semantics_FreeInductiveAlgebra(builtin);
+if (lean_io_result_is_error(res)) return res;
+lean_dec_ref(res);
+return lean_io_result_mk_ok(lean_box(0));
+}
+#ifdef __cplusplus
+}
+#endif
